src/axiomatic/PFtoA.v
@@ -867,60 +867,60 @@ Proof.
         rewrite List.app_length, Nat.add_1_r.
         ii. inv EID. inv REL.
         * admit. (* ctrl should be local *)
-        * (* TODO: move *)
-          Lemma addr_po_step ex:
-            (ex.(Execution.addr) ⨾ Execution.po) =
-            ((ex.(Execution.addr) ⨾ Execution.po) ∪ ex.(Execution.addr)) ⨾
-                                                                         Execution.po_adj.
-          Proof.
-            rewrite ? (union_seq' Execution.po_adj), ? seq_assoc, ? union_assoc.
-            rewrite Execution.po_po_adj at 1.
-            rewrite (clos_refl_union Execution.po), union_seq, eq_seq.
-            rewrite ? (seq_union' (Execution.po ⨾ Execution.po_adj) Execution.po_adj), ? seq_assoc, ? union_assoc.
-            refl.
-          Qed.
+        (* * (* TODO: move *) *)
+        (*   Lemma addr_po_step ex: *)
+        (*     (ex.(Execution.addr) ⨾ Execution.po) = *)
+        (*     ((ex.(Execution.addr) ⨾ Execution.po) ∪ ex.(Execution.addr)) ⨾ *)
+        (*                                                                  Execution.po_adj. *)
+        (*   Proof. *)
+        (*     rewrite ? (union_seq' Execution.po_adj), ? seq_assoc, ? union_assoc. *)
+        (*     rewrite Execution.po_po_adj at 1. *)
+        (*     rewrite (clos_refl_union Execution.po), union_seq, eq_seq. *)
+        (*     rewrite ? (seq_union' (Execution.po ⨾ Execution.po_adj) Execution.po_adj), ? seq_assoc, ? union_assoc. *)
+        (*     refl. *)
+        (*   Qed. *)
           
-          rewrite addr_po_step in H.
+        (*   rewrite addr_po_step in H. *)
           
-          (*TODO: move *)
-          Lemma step r eid tid n:
-            (r ⨾ Execution.po_adj) eid (tid, S n) = r eid (tid, n).
-          Proof.
-            propext. econs; i.
-            - inv H. des. inv H1. destruct x. ss. inv N. auto.
-            - econs. split; eauto.
-          Qed.
+        (*   (*TODO: move *) *)
+        (*   Lemma step r eid tid n: *)
+        (*     (r ⨾ Execution.po_adj) eid (tid, S n) = r eid (tid, n). *)
+        (*   Proof. *)
+        (*     propext. econs; i. *)
+        (*     - inv H. des. inv H1. destruct x. ss. inv N. auto. *)
+        (*     - econs. split; eauto. *)
+        (*   Qed. *)
 
-          rewrite step in H.
-          inv H.
-          { eapply VCAP; eauto. econs; eauto. econs 2; eauto. }
-          { (* TODO: move *)
-            Lemma addr_eid
-                  p ex (PRE: Valid.pre_ex p ex)
-                  eid tid eid2
-                  (ADDR: ex.(Execution.addr) eid (tid, eid2)):
-              exists eid1, eid = (tid, eid1).
-            Proof.
-            Admitted.
+        (*   rewrite step in H. *)
+        (*   inv H. *)
+        (*   { eapply VCAP; eauto. econs; eauto. econs 2; eauto. } *)
+        (*   { (* TODO: move *) *)
+        (*     Lemma addr_eid *)
+        (*           p ex (PRE: Valid.pre_ex p ex) *)
+        (*           eid tid eid2 *)
+        (*           (ADDR: ex.(Execution.addr) eid (tid, eid2)): *)
+        (*       exists eid1, eid = (tid, eid1). *)
+        (*     Proof. *)
+        (*     Admitted. *)
 
-            exploit addr_eid; eauto. i. des. subst.
-            exploit ADDR; eauto; ss.
-            { rewrite List.app_length. ss. clear. lia. }
-            i.
+        (*     exploit addr_eid; eauto. i. des. subst. *)
+        (*     exploit ADDR; eauto; ss. *)
+        (*     { rewrite List.app_length. ss. clear. lia. } *)
+        (*     i. *)
 
-            (* TODO: move *)
-            Lemma addr_inv
-                  p mem tid tr aeu atr wl rl covl vextl
-                  eid1 eid2
-                  (SIM: sim_trace p mem tid tr (aeu::atr) wl rl covl vextl)
-                  (EID2: eid2 >= List.length aeu.(AExecUnit.local).(ALocal.labels))
-                  (ADDR: aeu.(AExecUnit.local).(ALocal.addr) eid1 eid2):
-              False.
-            Proof.
-            Admitted.
+        (*     (* TODO: move *) *)
+        (*     Lemma addr_inv *)
+        (*           p mem tid tr aeu atr wl rl covl vextl *)
+        (*           eid1 eid2 *)
+        (*           (SIM: sim_trace p mem tid tr (aeu::atr) wl rl covl vextl) *)
+        (*           (EID2: eid2 >= List.length aeu.(AExecUnit.local).(ALocal.labels)) *)
+        (*           (ADDR: aeu.(AExecUnit.local).(ALocal.addr) eid1 eid2): *)
+        (*       False. *)
+        (*     Proof. *)
+        (*     Admitted. *)
 
-            exploit addr_inv; eauto. ss.
-          }
+        (*     exploit addr_inv; eauto. ss. *)
+        (*   } *)
       + rewrite List.app_length, Nat.add_1_r.
         i. rewrite sim_local_vrel_step. rewrite inverse_step.
         rewrite ? inverse_union. ii. des.
@@ -1021,20 +1021,84 @@ Proof.
       + admit. (* promise *)
     - (* if *)
       inv LC0. inv ASTATE_STEP; inv ALOCAL_STEP; ss; inv EVENT; ss. splits.
-      + econs; ss; try by apply L.
-      + econs; ss; try by apply L.
-
-        (* TODO: move *)
-        Lemma sim_view_le
-              (vext:eidT -> Time.t) (v1 v2:Time.t) (eids:eidT -> Prop)
-              (LE: le v1 v2)
-              (SIM: sim_view vext v1 eids):
-          sim_view vext v2 eids.
-        Proof.
-          ii. etrans; eauto.
-        Qed.
-
-        eapply sim_view_le; [apply join_l|]. apply L.
+      econs; ss.
+      { econs; ss. apply L. }
+      destruct L.(LC). ss. econs; ss.
+      + rewrite List.app_length, Nat.add_1_r.
+        i. rewrite sim_local_coh_step. rewrite inverse_step.
+        rewrite inverse_union. ii. des; [apply COH0|]; eauto.
+        inv EID. inv REL. inv H. inv H0. inv H2.
+        apply Label.is_writing_inv in LABEL. des. subst. inv H1.
+        * exploit EX2.(LABELS); eauto; ss; cycle 1.
+          { rewrite List.nth_error_app2, Nat.sub_diag; ss. }
+          { rewrite List.app_length. s. lia. }
+        * inv H. exploit RF2; eauto. i. des.
+          exploit EX2.(LABELS); eauto; ss; cycle 1.
+          { rewrite List.nth_error_app2, Nat.sub_diag; ss. }
+          { rewrite List.app_length. s. lia. }
+      + rewrite List.app_length, Nat.add_1_r.
+        i. rewrite sim_local_vrp_step. rewrite inverse_step.
+        rewrite ? inverse_union. ii. des.
+        * exploit VRP; eauto.
+        * inv EID. inv REL. inv H. inv H1. inv H. inv H2. inv H3.
+          exploit EX2.(LABELS); eauto; ss.
+          { rewrite List.app_length. s. lia. }
+          rewrite List.nth_error_app2, Nat.sub_diag; ss. i. simplify. ss.
+        * inv EID. inv REL. inv H. inv H1. inv H. inv H2. inv H3.
+          exploit EX2.(LABELS); eauto; ss.
+          { rewrite List.app_length. s. lia. }
+          rewrite List.nth_error_app2, Nat.sub_diag; ss. i. simplify. ss.
+        * inv EID. inv REL. inv H. inv H1. inv H2.
+          exploit EX2.(LABELS); eauto; ss.
+          { rewrite List.app_length. s. lia. }
+          { rewrite List.nth_error_app2, Nat.sub_diag; ss. }
+        * inv EID. inv REL. inv H0. destruct l; ss.
+          exploit EX2.(LABELS); eauto; ss.
+          { rewrite List.app_length. s. lia. }
+          { rewrite List.nth_error_app2, Nat.sub_diag; ss. }
+      + rewrite List.app_length, Nat.add_1_r.
+        i. rewrite sim_local_vwp_step. rewrite inverse_step.
+        rewrite ? inverse_union. ii. des.
+        * exploit VWP; eauto.
+        * inv EID. inv REL. inv H. inv H1. inv H. inv H2. inv H3.
+          exploit EX2.(LABELS); eauto; ss.
+          { rewrite List.app_length. s. lia. }
+          rewrite List.nth_error_app2, Nat.sub_diag; ss. i. simplify. ss.
+        * inv EID. inv REL. inv H. inv H1. inv H. inv H2. inv H3.
+          exploit EX2.(LABELS); eauto; ss.
+          { rewrite List.app_length. s. lia. }
+          rewrite List.nth_error_app2, Nat.sub_diag; ss. i. simplify. ss.
+        * inv EID. inv REL. inv H0. destruct l; ss.
+          exploit EX2.(LABELS); eauto; ss.
+          { rewrite List.app_length. s. lia. }
+          { rewrite List.nth_error_app2, Nat.sub_diag; ss. }
+      + rewrite List.app_length, Nat.add_1_r.
+        i. rewrite sim_local_vrm_step. rewrite inverse_step.
+        rewrite ? inverse_union. ii. des.
+        * exploit VRM; eauto.
+        * inv EID. inv REL. inv H0. destruct l; ss.
+          exploit EX2.(LABELS); eauto; ss; cycle 1.
+          { rewrite List.nth_error_app2, Nat.sub_diag; ss. }
+          { rewrite List.app_length. s. lia. }
+      + rewrite List.app_length, Nat.add_1_r.
+        i. rewrite sim_local_vwm_step. rewrite inverse_step.
+        rewrite ? inverse_union. ii. des.
+        * exploit VWM; eauto.
+        * inv EID. inv REL. inv H0. destruct l; ss.
+          exploit EX2.(LABELS); eauto; ss; cycle 1.
+          { rewrite List.nth_error_app2, Nat.sub_diag; ss. }
+          { rewrite List.app_length. s. lia. }
+      + admit. (* vcap *)
+      + rewrite List.app_length, Nat.add_1_r.
+        i. rewrite sim_local_vrel_step. rewrite inverse_step.
+        rewrite ? inverse_union. ii. des.
+        * exploit VREL; eauto.
+        * inv EID. inv REL. inv H0. destruct l; ss.
+          exploit EX2.(LABELS); eauto; ss.
+          { rewrite List.app_length. s. lia. }
+          { rewrite List.nth_error_app2, Nat.sub_diag; ss. }
+      + admit. (* fwdbank *)
+      + admit. (* promise *)
     - (* dowhile *)
       inv ASTATE_STEP; inv ALOCAL_STEP; ss; inv EVENT; ss. splits.
       + econs; ss; try by apply L.
@@ -1334,7 +1398,9 @@ Proof.
         - exploit Valid.ob_read_read_po; eauto. i.
           right. left. splits; eauto.
         - right. right. splits; eauto.
-        - inv LABEL1. }
+        - inv LABEL1.
+        - inv LABEL1.
+}
     + des.
       * left. etrans; eauto.
       * left. eapply le_lt_trans; eauto.
@@ -1378,13 +1444,12 @@ Proof.
   exploit TERMINAL; eauto. i. des. inv REL. inv x. congr.
 Grab Existential Variables.
 { (* external *)
-  ii. exploit Valid.ob_cycle; eauto. i. des.
-  - clear - EXTERNAL NONBARRIER.
-    exploit EXTERNAL; eauto. i. des.
-    + inv x; lia.
-    + inv x0. lia.
-    + inv x0. inv x1. rewrite EID in EID0. inv EID0. destruct l0; ss; congr.
-  - exploit Valid.barrier_ob_po; eauto. i. inv x1. lia.
+  ii. exploit Valid.ob_cycle; eauto. i. des. rename x1 into NONBARRIER.
+  clear - EXTERNAL NONBARRIER.
+  exploit EXTERNAL; eauto. i. des.
+  - inv x; lia.
+  - inv x0. lia.
+  - inv x0. inv x1. rewrite EID in EID0. inv EID0. destruct l0; ss; congr.
 }
 { (* internal *)
   clear - INTERNAL.
