src/axiomatic/PFtoALocal.v
@@ -354,7 +354,9 @@ Proof.
     + econs; ss.
       exploit sim_rmap_weak_expr; eauto. intro X. inv X.
       inv VAL. rewrite <- H0. ss.
-    + inv LOCAL1; [econs 1|econs 2]; eauto.
+    + inv LOCAL1; [econs 1|econs 2]; eauto; ss.
+      rewrite List.nth_error_app1; eauto.
+      eapply List.nth_error_Some. ii. congr.
   - eexists _, (AExecUnit.mk (State.mk _ _) _). splits; ss.
     + econs 7. ss.
     + econs; ss.
@@ -804,7 +806,7 @@ Proof.
         { subst. inv REL. inv Y. }
         eapply IH.(PO); eauto.
     }
-    { (* isb *)
+    { (* dmb *)
       inv STEP. inv ASTATE_STEP. ss. inv EVENT. econs; ss.
       - i. exploit IH.(WPROP1); eauto. s. i. des; [left|right]; esplits; eauto.
         eapply nth_error_app_mon. eauto.
@@ -824,7 +826,24 @@ Proof.
         eapply IH.(PO); eauto.
     }
   }
-  { (* internal *)
-    inv LOCAL; ss. inv LC. inv EVENT. econs; ss; try by apply IH.
+  { (* control *)
+    inv LOCAL; ss. inv LC. inv STATE0. inv ASTATE_STEP. ss. inv EVENT.
+    econs; ss.
+    - i. exploit IH.(WPROP1); eauto. s. i. des; [left|right]; esplits; eauto.
+      eapply nth_error_app_mon. eauto.
+    - i. exploit IH.(WPROP2); eauto.
+      apply nth_error_snoc_inv in GET. des; eauto. congr.
+    - i. exploit IH.(WPROP3); eauto. i. des. esplits; eauto.
+      eapply nth_error_app_mon. eauto.
+    - eapply IH.(WPROP4).
+    - i. exploit IH.(RPROP1); eauto.
+      apply nth_error_snoc_inv in GET. des; eauto. congr.
+    - i. exploit IH.(RPROP2); eauto. s. i. des. esplits; eauto.
+      eapply nth_error_app_mon. eauto.
+    - i. apply nth_error_snoc_inv in LABEL1. des; cycle 1.
+      { subst. inv REL. inv X. }
+      apply nth_error_snoc_inv in LABEL2. des; cycle 1.
+      { subst. inv REL. inv Y. }
+      eapply IH.(PO); eauto.
   }
 Admitted.
